src/tls/Model.AEAD.fst
@@ -1,0 +1,98 @@
+module Model.AEAD
+
+module U8 = FStar.UInt8
+module Seq = FStar.Seq
+module SC = Spec.AEAD
+module U32 = FStar.UInt32
+module HS = FStar.HyperStack
+module HST = FStar.HyperStack.ST
+module G = FStar.Ghost
+module F = Flags
+module B = LowStar.Buffer
+module MDM = FStar.Monotonic.DependentMap
+
+friend Lib.IntTypes // because Spec.uint8 is a secret integer type but miTLS is using FStar UInt8
+
+noextract
+inline_for_extraction
+let entry (a: SC.supported_alg): Tot eqtype =
+  [@inline_let]
+  let t = SC.iv a in
+  t
+
+let table
+  (a: SC.supported_alg)
+  (kv: SC.kv a)
+  (phi: plain_pred)
+: Tot Type0
+= MDM.t HS.root (entry a) (fun iv -> (plain: SC.plain a { phi plain })) (fun _ -> True)
+
+noeq
+type state (a: SC.supported_alg) (phi: plain_pred) = {
+  kv: SC.kv a;
+  table: (if F.ideal_AEAD then table a kv phi else unit)
+}
+
+let state_kv
+  (#a: SC.supported_alg) (#phi: plain_pred)
+  (s: state a phi)
+: Tot (SC.kv a)
+= s.kv
+
+let state_table
+  (#a: SC.supported_alg) (#phi: plain_pred)
+  (s: state a phi)
+: Pure (table a (state_kv s) phi)
+  (requires (Flags.ideal_AEAD == true))
+  (ensures (fun _ -> True))
+= s.table <: table a (state_kv s) phi
+
+let invariant (#a: SC.supported_alg) (#phi: plain_pred) (h: HS.mem) (s: state a phi) : GTot Type0 =
+  if F.ideal_AEAD
+  then
+    h `HS.contains` state_table s
+  else
+    True
+
+let footprint
+  #a #phi s
+= if F.ideal_AEAD
+  then
+    B.loc_mreference (state_table s)
+  else
+    B.loc_none
+
+let frame_invariant
+  #a #phi h s l h'
+= if F.ideal_AEAD
+  then
+    B.modifies_mreference_elim (state_table s) l h h' // FIXME: WHY WHY WHY do I need to call this lemma by hand?
+  else
+    ()
+
+let encrypt
+  #a #phi s iv plain
+= if F.ideal_AEAD
+  then begin
+    let h = HST.get () in
+    let tbl = state_table s in
+    assume (~ (MDM.defined tbl iv h)); // cryptographic assumption
+    MDM.extend tbl iv plain;
+    let h' = HST.get () in
+    B.modifies_loc_regions_intro (Set.singleton (HS.frameOf tbl)) h h' ;
+    B.modifies_loc_addresses_intro (HS.frameOf tbl) (Set.singleton (HS.as_addr tbl)) B.loc_none h h' ;
+    Seq.create (SC.cipher_length plain) 0uy
+  end else
+    SC.encrypt (state_kv s) iv Seq.empty plain
+
+let decrypt
+  #a #phi s iv cipher
+= if F.ideal_AEAD
+  then begin
+    match MDM.lookup (state_table s) iv with
+    | None -> None
+    | Some plain -> Some plain
+  end else
+    match SC.decrypt (state_kv s) iv Seq.empty cipher with
+    | None -> None
+    | Some plain -> Some plain
