src/tls/Model.AEAD.fsti
@@ -1,0 +1,76 @@
+module Model.AEAD
+
+module U8 = FStar.UInt8
+module Seq = FStar.Seq
+module SC = Spec.AEAD
+module U32 = FStar.UInt32
+module HS = FStar.HyperStack
+module HST = FStar.HyperStack.ST
+module G = FStar.Ghost
+module F = Flags
+module B = LowStar.Buffer
+
+(* THIS MODULE MUST NOT BE EXTRACTED *)
+
+type plain_pred = (plain: Seq.seq SC.uint8) -> Tot Type0
+
+val state (a: SC.supported_alg) (phi: plain_pred) : Tot Type0
+
+val state_kv
+  (#a: SC.supported_alg) (#phi: plain_pred)
+  (s: state a phi)
+: Tot (SC.kv a)
+
+val invariant (#a: SC.supported_alg) (#phi: plain_pred) (h: HS.mem) (s: state a phi) : GTot Type0
+
+val footprint (#a: SC.supported_alg) (#phi: plain_pred) (s: state a phi) : GTot B.loc
+
+val frame_invariant
+  (#a: SC.supported_alg) (#phi: plain_pred) (h: HS.mem) (s: state a phi)
+  (l: B.loc) (h' : HS.mem)
+: Lemma
+  (requires (B.modifies l h h' /\ B.loc_disjoint l (footprint s) /\ invariant h s))
+  (ensures (invariant h' s))
+
+val encrypt
+  (#a: SC.supported_alg)
+  (#phi: plain_pred)
+  (s: state a phi) // key
+  (iv: SC.iv a)
+  (plain: SC.plain a)
+: HST.ST (SC.encrypted plain)
+  (requires (fun h ->
+    Flags.model == true /\
+    invariant h s /\
+    phi plain
+  ))
+  (ensures (fun h cipher h' -> 
+    B.modifies (footprint s) h h' /\
+    Seq.length cipher <= SC.max_length a + SC.tag_length a /\
+    invariant h' s /\
+    (Flags.ideal_AEAD == false ==> (
+      SC.encrypt (state_kv s) iv Seq.empty plain == cipher /\
+      HST.equal_domains h h' // to go to the Stack effect
+  ))))
+
+val decrypt
+  (#a: SC.supported_alg)
+  (#phi: plain_pred)
+  (s: state a phi) // key
+  (iv: SC.iv a)
+  (cipher: SC.cipher a { Seq.length cipher <= SC.max_length a + SC.tag_length a })
+: HST.ST (option (SC.plain a))
+  (requires (fun h ->
+    Flags.model == true /\
+    invariant h s
+  ))
+  (ensures (fun h res h' ->
+    B.modifies (footprint s) h h' /\
+    (Flags.ideal_AEAD == false ==> HST.equal_domains h h') /\ // to go to the Stack effect
+    begin match res with
+    | None -> True
+    | Some plain ->
+      invariant h' s /\
+      Flags.ideal_AEAD == true ==> phi plain
+    end
+  ))
